lib/ModuRes/Util.v
@@ -1,5 +1,6 @@
 Require Import Ssreflect.ssreflect.
 Require Import Setoid SetoidClass.
+Require Import List.
 
 Ltac find_rewrite1 t0 t1 := match goal with
                             | H: t0 = t1 |- _ => rewrite-> H
@@ -19,3 +20,20 @@ Ltac split_conjs := repeat (match goal with [ |- _ /\ _ ] => split end).
 
 (* TODO: Is this already defined somewhere? *)
 Class DecEq (T : Type) := dec_eq : forall (t1 t2: T), {t1 = t2} + {t1 <> t2}.
+
+(* Stuff that ought to be in the stdlib... *)
+Lemma NoDup_app3 {T} (l1 l2 l3: list T):
+  NoDup (l1 ++ l2 ++ l3) -> NoDup (l2 ++ l1 ++ l3).
+Proof.
+  revert l2 l3. induction l1; induction l2; intro l3; simpl; try tauto; [].
+  move=>Hndup. change (NoDup (a0 :: l2 ++ (a::nil) ++ l1 ++ l3)).
+  apply NoDup_cons; last first.
+  - apply IHl2. eapply NoDup_remove_1. eassumption.
+  - rewrite app_comm_cons in Hndup. apply NoDup_remove_2 in Hndup.
+    move=>Hin. apply Hndup. clear -Hin. rewrite !in_app_iff. rewrite ->!in_app_iff in Hin.
+    destruct Hin as [Hin|[[Hin|[]]|[Hin|Hin]]].
+    + right. left. assumption.
+    + left. left. assumption.
+    + left. right. assumption.
+    + right. right. assumption.
+Qed.
